Towards value optimizations.

ValueOpts.v
@@ -124,17 +124,48 @@ Definition sem_entails Gamma Γ' := forall E, satisfiesAll E Gamma -> satisfiesA
 Definition freeVars (gamma:exp * exp) := 
   let (e,e'):= gamma in Exp.freeVars e ∪ Exp.freeVars e'.
 
+Definition domain (gamma:exp * exp) := 
+  let (e,e'):= gamma in Exp.freeVars e.
+
 Definition eqns_freeVars (Gamma:eqns) := list_union (List.map freeVars Gamma).
 
 Definition entails Gamma Γ' := (forall E, satisfiesAll E Gamma -> satisfiesAll E Γ') 
 /\ eqns_freeVars Γ' ⊆ eqns_freeVars Gamma. 
 
+Definition onvLe X (E E':onv X)
+:= forall x v, E x = Some v -> E' x = Some v.
+
 Definition moreDefined Gamma Γ' e e' := 
-  forall E E', satisfiesAll E Gamma -> satisfiesAll E' Γ' -> fstNoneOrR eq (exp_eval E e) (exp_eval E' e').
+  forall E E', onvLe E E'
+          -> satisfiesAll E Gamma 
+          -> satisfiesAll E' Γ'
+          -> fstNoneOrR eq (exp_eval E e) (exp_eval E' e').
+
+Lemma exp_eval_onvLe e E E' v
+: onvLe E E' 
+  -> exp_eval E e = Some v
+  -> exp_eval E' e = Some v.
+Proof.
+  intros. general induction e; simpl in * |- *; eauto.
+  simpl in H0. rewrite H0. eapply H in H0. eauto.
+  monad_inv H0. rewrite EQ, EQ1.
+  erewrite IHe1, IHe2; eauto.
+Qed.
+
+Instance moreDefined_refl Gamma Γ'
+: Reflexive (moreDefined Gamma Γ').
+Proof.
+  hnf; intros; hnf; intros.
+  case_eq (exp_eval E x); intros.
+  erewrite exp_eval_onvLe; eauto. constructor; eauto.
+  constructor.
+Qed.
 
 Definition moreDefinedArgs Gamma Γ' Y Y' := 
-  forall E E', satisfiesAll E Gamma -> satisfiesAll E' Γ' -> 
-          fstNoneOrR eq (omap (exp_eval E) Y) (omap (exp_eval E') Y').
+  forall E E', onvLe E E'
+          -> satisfiesAll E Gamma 
+          -> satisfiesAll E' Γ' 
+          -> fstNoneOrR eq (omap (exp_eval E) Y) (omap (exp_eval E') Y').
 
 (*Definition moreDefined Gamma Γ' e e' := 
   forall E, satisfies E Gamma -> forall E', satisfies E' Γ' -> moreDef (exp_eval E e) (exp_eval E' e').*)
@@ -152,54 +183,58 @@ Definition subst_eqns (ϱ : env exp) (G:list eqn) :=
 Definition sid := fun x => Var x.
 
 
-Inductive eqn_sound : list (params*eqns*eqns*eqns*eqns) 
+Inductive eqn_sound : list (params*set var*eqns*eqns*eqns*eqns) 
                       -> stmt 
                       -> ann (eqns) 
                       -> ann (eqns) 
+                      -> ann (set var * set var)
                       -> ann (list exp) 
                       -> Prop :=
-| EqnOpr x Lv b e Gamma al Γ' (al':ann (eqns)) e' cl
-  : eqn_sound Lv b al al' cl
+| EqnOpr x Lv b e Gamma al Γ' (al':ann (eqns)) e' cl G G' ang
+  : eqn_sound Lv b al al' ang cl 
     (* make sure the rest conforms to the new assignment *)
     -> entails ((Var x,e)::Gamma) (getAnn al)
     -> entails ((Var x,e')::Γ') (getAnn al')
     -> moreDefined Gamma Γ' e e'
-    -> Exp.freeVars e' ⊆ eqns_freeVars Γ'
-    -> eqn_sound Lv (stmtExp x e b) (ann1 Gamma al) (ann1 Γ' al') (ann1 (e'::nil) cl)
-| EqnIf Lv e e' b1 b2 Gamma Γ' al1 al2 al1' al2' cl1 cl2
-  : eqn_sound Lv b1 al1 al1' cl1
-  -> eqn_sound Lv b2 al2 al2' cl2
+    -> Exp.freeVars e' ⊆ G
+    -> eqn_sound Lv (stmtExp x e b) (ann1 Gamma al) (ann1 Γ' al')
+                (ann1 (G,G') ang) (ann1 (e'::nil) cl)
+| EqnIf Lv e e' b1 b2 Gamma Γ' al1 al2 al1' al2' cl1 cl2 G G' ang1 ang2
+  : eqn_sound Lv b1 al1 al1' ang1 cl1
+  -> eqn_sound Lv b2 al2 al2' ang2 cl2
  (* TODO: include information about condition *)
   -> entails Gamma (getAnn al1)
   -> entails Gamma (getAnn al2)
   -> entails Γ' (getAnn al1')
   -> entails Γ' (getAnn al2')
   -> moreDefined Gamma Γ' e e'
-  -> eqn_sound Lv (stmtIf e b1 b2) (ann2 Gamma al1 al2) (ann2 Γ' al1' al2') (ann2 (e'::nil) cl1 cl2)
-| EqnGoto l Y Y' Lv Gamma Γ' Z Γf Γf' EqS EqS'
-  : get Lv (counted l) (Z,Γf, EqS, Γf',EqS')
+  -> eqn_sound Lv (stmtIf e b1 b2) (ann2 Gamma al1 al2) (ann2 Γ' al1' al2') 
+              (ann2 (G,G') ang1 ang2) (ann2 (e'::nil) cl1 cl2)
+| EqnGoto l Y Y' Lv Gamma Γ' Z Γf Γf' EqS EqS' Gf G G'
+  : get Lv (counted l) (Z,Gf,Γf, EqS, Γf',EqS')
     -> length Y = length Y'
     -> entails Gamma (subst_eqns (sid [Z <-- Y]) EqS)
     -> entails Γ' (subst_eqns (sid [Z <-- Y']) EqS')
     -> moreDefinedArgs Gamma Γ' Y Y'
-    -> eqn_sound Lv (stmtGoto l Y) (ann0 Gamma) (ann0 Γ') (ann0 Y')
-| EqnReturn Lv e e' Gamma Γ'
+    -> eqn_sound Lv (stmtGoto l Y) (ann0 Gamma) (ann0 Γ') (ann0 (G,G')) (ann0 Y')
+| EqnReturn Lv e e' Gamma Γ' G G'
   : moreDefined Gamma Γ' e e'
-    -> eqn_sound Lv (stmtReturn e) (ann0 Gamma) (ann0 Γ') (ann0 (e'::nil))
-| EqnLet Lv s Z b Gamma Γ' EqS EqS' als alb als' alb' cls clb
-  : eqn_sound ((Z,Gamma, EqS, Γ', EqS')::Lv) s als als' cls
-  -> eqn_sound ((Z,Gamma, EqS, Γ', EqS')::Lv) b alb alb' clb
+    -> eqn_sound Lv (stmtReturn e) (ann0 Gamma) (ann0 Γ') (ann0 (G,G')) (ann0 (e'::nil))
+| EqnLet Lv s Z b Gamma Γ' EqS EqS' als alb als' alb' cls clb G G' angs angb
+  : eqn_sound ((Z, G, Gamma, EqS, Γ', EqS')::Lv) s als als' angs cls
+  -> eqn_sound ((Z, G ,Gamma, EqS, Γ', EqS')::Lv) b alb alb' angb clb
   -> entails (EqS ++ Gamma) (getAnn als)
   -> entails Gamma (getAnn alb)
   -> entails (EqS' ++ Γ') (getAnn als')
   -> entails Γ' (getAnn alb')
-  -> eqns_freeVars EqS ⊆ eqns_freeVars Gamma ++ of_list Z
-  -> eqns_freeVars EqS' ⊆ eqns_freeVars Γ' ++ of_list Z
-  -> eqn_sound Lv (stmtLet Z s b) (ann2 Gamma als alb) (ann2 Γ' als' alb') (ann2 nil cls clb).
+  -> eqns_freeVars EqS ⊆ G ++ of_list Z
+  -> eqns_freeVars EqS' ⊆ G ++ of_list Z
+  -> eqn_sound Lv (stmtLet Z s b) (ann2 Gamma als alb) (ann2 Γ' als' alb') 
+              (ann2 (G,G') angs angb) (ann2 nil cls clb).
 
 Fixpoint compile (s:stmt) (a:ann (list exp)) :=
   match s, a with
-    | stmtExp x _ s, ann1 (e'::nil) an => 
+    | stmtExp x _ s, ann1 (e'::nil) an =>
       stmtExp x e' (compile s an)
     | stmtIf _ s t, ann2 (e'::nil) ans ant => 
       stmtIf e' (compile s ans) (compile t ant)
@@ -211,41 +246,39 @@ Fixpoint compile (s:stmt) (a:ann (list exp)) :=
     | s, _ => s
   end.
 
-Definition onvLe X (E E':onv X)
-:= forall x v, E x = Some v -> E' x = Some v.
 
 
-Definition ArgRel E E' (G:list var*eqns*eqns*eqns*eqns) (VL VL': list val) : Prop := 
-  let '(Z, Gamma, EqS, Γ', EqS') := G in
+Definition ArgRel E E' (a:list var*set var*eqns*eqns*eqns*eqns) (VL VL': list val) : Prop := 
+  let '(Z, G, Gamma, EqS, Γ', EqS') := a in
   length Z = length VL 
-  /\ length VL = length VL' 
+  /\ VL = VL' 
   /\ satisfiesAll (E[Z <-- List.map Some VL]) (EqS ++ Gamma)
   /\ satisfiesAll (E'[Z <-- List.map Some VL']) (EqS' ++ Γ').
 
-Definition ParamRel (G:params*eqns*eqns*eqns*eqns) (Z Z' : list var) : Prop := 
-  let '(Zb, Gamma, EqS, Γ', EqS') := G in  
+Definition ParamRel (a:params*set var*eqns*eqns*eqns*eqns) (Z Z' : list var) : Prop := 
+  let '(Zb, G, Gamma, EqS, Γ', EqS') := a in  
   Z = Z' /\ Zb = Z.
 
-Definition BlockRel (lv:set var) (V V':onv val) (G:params*eqns*eqns*eqns*eqns) (b b':F.block) : Prop := 
-  let '(Zb, Gamma, EqS, Γ', EqS') := G in  
-  eqns_freeVars Gamma ∩ of_list Zb [=] {}
-  /\ eqns_freeVars Γ' ∩ of_list Zb [=] {}
-  /\ eqns_freeVars EqS ⊆ eqns_freeVars Gamma ∪ of_list Zb
-  /\ eqns_freeVars EqS' ⊆ eqns_freeVars Γ' ∪ of_list Zb
+Definition BlockRel (G':set var) (V V':onv val) (a:params*set var*eqns*eqns*eqns*eqns) (b b':F.block) : Prop := 
+  let '(Zb, G, Gamma, EqS, Γ', EqS') := a in  
+  G ∩ of_list Zb [=] {}
+  /\ G ⊆ G'
+  /\ eqns_freeVars EqS ⊆ G ∪ of_list Zb
+  /\ eqns_freeVars EqS' ⊆ G ∪ of_list Zb
   /\ satisfiesAll (F.block_E b) Gamma
   /\ satisfiesAll (F.block_E b') Γ'
-  /\ agree_on eq (eqns_freeVars Gamma) (F.block_E b) V
-  /\ agree_on eq (eqns_freeVars Γ') (F.block_E b') V'
-  /\ eqns_freeVars Gamma ⊆ lv
-  /\ eqns_freeVars Γ' ⊆ lv.
+  /\ agree_on eq G (F.block_E b) V
+  /\ agree_on eq G (F.block_E b') V'
+  /\ eqns_freeVars Gamma ⊆ G
+  /\ eqns_freeVars Γ' ⊆ G.
 
-Instance AR lv V V' : ApxRelation (params*eqns*eqns*eqns*eqns) := {
+Instance AR lv V V' : ApxRelation (params*set var*eqns*eqns*eqns*eqns) := {
   ArgRel := ArgRel;
   ParamRel := ParamRel;
   BlockRel := BlockRel lv V V'
 }.
 intros. hnf in H. hnf in H0.
-destruct a as [[[[]]]]; dcr; split; congruence.
+destruct a as [[[[[]]]]]; dcr; split; congruence.
 Defined.
 
 (* problem is Gamma that satisfies nothing 
@@ -282,7 +315,7 @@ Proof.
     hnf; intros. cset_tac; intuition.
 Qed.
 
-Lemma eqn_freeVars_incl (Gamma:eqns) gamma n
+Lemma eqns_freeVars_incl (Gamma:eqns) gamma n
   : get Gamma n gamma
     -> freeVars gamma ⊆ eqns_freeVars Gamma.
 Proof.
@@ -362,11 +395,17 @@ Proof.
   symmetry. 
   erewrite <- minus_inane_set.
   eapply update_with_list_agree_minus; eauto. reflexivity.
-  exfalso; admit. inv X; eauto.
+  exploit eqns_freeVars_incl; eauto.
+  destruct gamma; simpl in *. rewrite <- H1. 
+  revert H1 X0; clear_all; cset_tac; intuition; exfalso; eauto.
+  inv X; eauto.
   erewrite <- minus_inane_set.
   symmetry.
   eapply update_with_list_agree_minus; eauto. reflexivity.
-  exfalso; admit. inv X; eauto.
+  exploit eqns_freeVars_incl; eauto.
+  destruct gamma; simpl in *. rewrite <- H1. 
+  revert H1 X0; clear_all; cset_tac; intuition; exfalso; eauto.
+  inv X; eauto.
 Qed.
 
 Lemma eval_exp_subst E y Y Z e
@@ -392,18 +431,8 @@ Proof.
   erewrite IHe2; eauto.
 Qed.
 
-Lemma exp_eval_onvLe e E E' v
-: onvLe E E' 
-  -> exp_eval E e = Some v
-  -> exp_eval E' e = Some v.
-Proof.
-  intros. general induction e; simpl in * |- *; eauto.
-  simpl in H0. rewrite H0. eapply H in H0. eauto.
-  monad_inv H0. rewrite EQ, EQ1.
-  erewrite IHe1, IHe2; eauto.
-Qed.
 
-Lemma agree_on_onvLe X `{OrderedType.OrderedType X} (V V':onv X) Z vl
+Lemma agree_on_onvLe {X} `{OrderedType.OrderedType X} (V V':onv X) Z vl
 : onvLe V V'
   -> onvLe (V [Z <-- vl]) (V' [Z <-- vl]).
 Proof.
@@ -438,7 +467,7 @@ Proof.
     eapply H5; eauto. eapply H2; eauto. 
 Qed.
 
-Lemma eqns_freeVars_incl Gamma Γ' G x e
+Lemma entails_freeVars_incl Gamma Γ' G x e
 : entails ((Var x, e)::Gamma) Γ'
   -> Exp.freeVars e ⊆ G
   -> eqns_freeVars Gamma ⊆ G
@@ -474,13 +503,13 @@ Proof.
   - rewrite <- H1. rewrite eqns_freeVars_add. cset_tac; intuition.
 Qed.
 
-Lemma satisfiesAll_subst V Gamma Γf Z EqS Y y bE
+Lemma satisfiesAll_subst V Gamma Γf Z EqS Y y bE G
 :  length Z = length Y
-   -> eqns_freeVars EqS ⊆ eqns_freeVars Γf ∪ of_list Z
-   -> eqns_freeVars Γf ∩ of_list Z [=] ∅
+   -> eqns_freeVars EqS ⊆ G ∪ of_list Z
+   -> G ∩ of_list Z [=] ∅
    -> entails Gamma (subst_eqns (sid [Z <-- Y]) EqS)
    -> satisfiesAll V Gamma
-   -> agree_on eq (eqns_freeVars Γf) V bE
+   -> agree_on eq G V bE
    -> ⎣y ⎦ = omap (exp_eval V) Y
    -> satisfiesAll bE Γf
    -> satisfiesAll (bE [Z <-- List.map Some y]) EqS.
@@ -500,7 +529,7 @@ Proof.
       eapply X.
       eapply update_with_list_agree; eauto.
       eapply agree_on_incl; eauto. 
-      exploit eqn_freeVars_incl; eauto. 
+      exploit eqns_freeVars_incl; eauto. 
       rewrite H0 in X0. simpl in X0.
       rewrite <- (minus_union_set _ _ _ H1); eauto.
       rewrite <- X0. eapply incl_minus_lr; cset_tac; intuition.
@@ -508,7 +537,7 @@ Proof.
       exploit omap_length; eauto. congruence.
       eapply update_with_list_agree; eauto.
       eapply agree_on_incl; eauto. 
-      exploit eqn_freeVars_incl; eauto. 
+      exploit eqns_freeVars_incl; eauto. 
       rewrite H0 in X0. simpl in X0.
       rewrite <- (minus_union_set _ _ _ H1); eauto.
       rewrite <- X0. eapply incl_minus_lr; cset_tac; intuition.
@@ -553,92 +582,112 @@ Proof.
     destruct gamma; simpl; cset_tac; intuition.
 Qed.
 
-Lemma sim_DVE r L L' V V' s LV eqns eqns' repl G G'
+Lemma sim_DVE r L L' V V' s LV eqns eqns' repl ang
 :
   satisfiesAll V (getAnn eqns) 
 -> satisfiesAll V' (getAnn eqns')
--> eqn_sound LV s eqns eqns' repl
--> simL' r (AR G V V') LV L L'
--> ssa G s G'
--> eqns_freeVars (getAnn eqns) ⊆ G
--> eqns_freeVars (getAnn eqns') ⊆ G
+-> eqn_sound LV s eqns eqns' ang repl
+-> simL' r (AR (fst (getAnn ang)) V V') LV L L'
+-> ssa s ang
+-> eqns_freeVars (getAnn eqns) ⊆ fst (getAnn ang)
+-> eqns_freeVars (getAnn eqns') ⊆ fst (getAnn ang)
+-> onvLe V V'
 -> paco2 (@psimapx F.state _ F.state _) r (L,V, s) (L',V', compile s repl).
 Proof.
   general induction s; simpl; invt eqn_sound; invt ssa; simpl in * |- *.
-  + unfold moreDefined in H16; exploit H16; eauto. inv X.
+  + exploiT moreDefined; eauto. inv X.
     - pfold. econstructor 3; try eapply star_refl; eauto. stuck.
     - pfold. econstructor; try eapply plusO.
       econstructor; eauto using eq_sym.
       econstructor; eauto using eq_sym.
       left. eapply IHs; eauto.
-      eapply H10.
-      eapply satisfiesAll_update; eauto.
-      eapply H12. eapply satisfiesAll_update; eauto.
-      eapply simL'_update; eauto.
-      intros. hnf in H8.
-      hnf. destruct x0 as [[[[] ?] ?] ?]. dcr. repeat (split; eauto).
-      symmetry. eapply agree_on_update_dead.
-      intro. eapply H13. eauto. symmetry; eauto.
-      symmetry. eapply agree_on_update_dead.
-      intro. eapply H13. eauto. symmetry; eauto.
-      cset_tac; intuition. cset_tac; intuition.
-      clear_all; firstorder.
-      eauto using eqns_freeVars_incl.
-      eapply eqns_freeVars_incl; eauto.
-      rewrite H17; eauto.
-  + unfold moreDefined in H19; exploit H19; eauto. inv X.
+      * eapply H11. eapply satisfiesAll_update; eauto.
+      * eapply H13. eapply satisfiesAll_update; eauto.
+      * eapply simL'_update; eauto.
+        intros. hnf in H9.
+        hnf. destruct x0 as [[[[[] ?] ?] ?] ?]. dcr. repeat (split; eauto).
+        rewrite H21. rewrite H16. simpl. clear_all; cset_tac; intuition.
+        symmetry. eapply agree_on_update_dead.
+        intro. eapply H15. eauto. 
+        symmetry; eauto. 
+        symmetry. eapply agree_on_update_dead.
+        intro. eapply H15. eauto. 
+        symmetry; eauto.
+        clear_all; firstorder.
+      * rewrite H21. simpl. eauto using entails_freeVars_incl.
+      * rewrite H21. eapply entails_freeVars_incl; eauto.
+      * hnf; intros. lud; eauto.
+  + exploiT moreDefined; eauto. inv X.
     - pfold. econstructor 3; try eapply star_refl; eauto. stuck.
     - pfold. case_eq (val2bool y); intros. 
       econstructor; try eapply plusO.
       econstructor; eauto using eq_sym.
       econstructor; eauto using eq_sym.
       left. eapply IHs1; eauto.
-      eapply H11; eauto.
-      eapply H14; eauto.
-      destruct H11. rewrite H16; eauto. 
-      destruct H14. rewrite H16; eauto.
-      econstructor; try eapply plusO.
-      econstructor 3; eauto using eq_sym.
-      econstructor 3; eauto using eq_sym.
-      left. eapply IHs2; try eapply H10; eauto.
-      eapply H12; eauto.
-      eapply H18; eauto.
-      destruct H12. rewrite H16; eauto.
-      destruct H18. rewrite H18; eauto.
+      * eapply H12; eauto.
+      * eapply H15; eauto.
+      * eapply simL'_update; eauto.
+        unfold SimApx.BlockRel.
+        destruct x as [[[[[] ?] ?] ?] ?]; simpl; intros; dcr. 
+        repeat (split; eauto).
+        rewrite H26; eauto.
+        clear_all; firstorder.
+      * inv H12. rewrite H26; eauto; simpl. rewrite H16; eauto. 
+      * inv H15. rewrite H26; eauto; simpl. rewrite H16; eauto. 
+      * econstructor; try eapply plusO.
+        econstructor 3; eauto using eq_sym.
+        econstructor 3; eauto using eq_sym.
+        left. eapply IHs2; try eapply H10; eauto.
+        eapply H13; eauto.
+        eapply H20; eauto.
+        eapply simL'_update; eauto.
+        unfold SimApx.BlockRel.
+        destruct x as [[[[[] ?] ?] ?] ?]; simpl; intros; dcr. 
+        repeat (split; eauto).
+        rewrite H27; eauto.
+        clear_all; firstorder.
+        inv H13. rewrite H16; eauto. rewrite H27; eauto.
+        inv H20. rewrite H16; eauto. rewrite H27; eauto.
   + destruct (get_dec L (counted l)) as [[[bE bZ bs]]|].
     (* hnf in H2. exploit H2; eauto. simpl in *. subst bZ. *)
     decide (length bZ = length Y).
-    hnf in H16. exploit H16; eauto. inv X.
+    exploiT moreDefinedArgs; eauto. inv X.
     - pfold. econstructor 3; try eapply star_refl. eauto. stuck.
     - edestruct AIR5_length; try eassumption; dcr.
       edestruct get_length_eq; try eassumption.
       edestruct AIR5_nth as [?[? [?]]]; try eassumption; dcr. 
       simpl in *. repeat get_functional; subst.
-      inv H25. hnf in H28; simpl in H28; dcr; subst.
-      eapply sim_drop_shift. eapply H31; eauto. hnf. simpl; repeat split. 
+      inv H26. hnf in H29; simpl in H29; dcr; subst.
+      eapply sim_drop_shift. eapply H32; eauto. hnf. simpl; repeat split. 
       exploit omap_length; eauto. unfold var in *. rewrite e. congruence.
-      intros. inv H10.
+      intros. inv H11.
       intros.       
-      hnf in H30; dcr. eauto. 
+      hnf in H31; dcr.
       eapply satisfiesAll_union; split; eauto.
-      eapply (@satisfiesAll_subst V Gamma Γf); eauto. symmetry; eauto.
+      eapply (@satisfiesAll_subst V Gamma Γf); eauto. 
+      symmetry; eauto.
       eapply satisfiesAll_update_dead; eauto. rewrite map_length.
-      exploit omap_length; eauto. congruence. simpl in *.
-      intros. inv H12.
+      exploit omap_length; eauto. congruence.
+      rewrite <- H19.
+      revert H19 H35; clear_all; cset_tac; intuition; exfalso; eauto.
+      simpl in *.
+      intros. inv H13.
       intros.       
-      hnf in H30; dcr. 
+      hnf in H31; dcr. 
       eapply satisfiesAll_union; split; eauto.
       simpl in *.
       eapply (@satisfiesAll_subst V' Γ' Γf'); 
-        try eapply H7; eauto using agree_on_sym.
+        try eapply H8; eauto.
       congruence. 
       symmetry; eauto.
       eapply satisfiesAll_update_dead; eauto. rewrite map_length. 
       exploit omap_length; eauto. congruence. 
+      rewrite <- H19.
+      revert H19 H37; clear_all; cset_tac; intuition; exfalso; eauto.
     - pfold. econstructor 3; try eapply star_refl. eauto. stuck; eauto.
       get_functional; subst. simpl in *. congruence.
     - pfold. econstructor 3; try eapply star_refl. eauto. stuck; eauto.
-  + simpl. hnf in H8; exploit H8; eauto. inv X; eauto.
+  + simpl. exploiT moreDefined; eauto. inv X; eauto.
     - pfold. econstructor 3; try eapply star_refl. simpl. congruence.
       stuck.
     - pfold. econstructor 2; try eapply star_refl. simpl. congruence.
@@ -647,50 +696,53 @@ Proof.
     econstructor; eauto.
     econstructor; eauto.
     simpl. left. eapply IHs2; eauto.
-    - eapply H12; eauto.
-    - eapply H15; eauto.
+    - eapply H13; eauto.
+    - eapply H16; eauto.
     - eapply simL_mon; eauto. eapply simL_extension'; eauto.
-      * hnf; intros. hnf in H6; dcr.
+      * eapply simL'_update; eauto.
+        unfold SimApx.BlockRel.
+        destruct x as [[[[[] ?] ?] ?] ?]; simpl; intros; dcr. 
+        repeat (split; eauto).
+        rewrite H28; eauto.
+        clear_all; firstorder.
+      * hnf; intros. hnf in H7; dcr.
         eapply IHs1; eauto.
-        eapply H11. eauto. 
-        eapply H13. eauto.
+        eapply H12. eauto. 
+        eapply H14. eauto.
         eapply simL'_update; eauto.
         unfold SimApx.BlockRel. intros. 
-        destruct x as [[[[] ?] ?] ?]; dcr. simpl in H6.
-        simpl. dcr.
-        split; eauto.
-        split; eauto.
-        split; eauto.
-        split; eauto.
-        split; eauto.
-        split; eauto.
-        split.
-        assert (eqns_freeVars e [=] eqns_freeVars e \ of_list Z) by admit.
-        rewrite H6. symmetry.
+        destruct x as [[[[[] ?] ?] ?] ?]; dcr. simpl in H7.
+        simpl. dcr. 
+        assert (sEQ: s [=] s \ of_list Z). {
+          assert (s ∩ of_list Z [=] ∅).
+          rewrite <- H20. rewrite H28 in H32.
+          revert H32 H20; simpl; clear_all; cset_tac; intuition; exfalso; eauto.
+          rewrite <- (minus_union_set _ _ _ H7).
+          clear_all; cset_tac; intuition.
+        }
+        repeat (split; eauto).
+        rewrite H32. rewrite H26. rewrite H28. simpl. eapply incl_right.
+        rewrite sEQ. symmetry.
         eapply update_with_list_agree_minus; eauto. rewrite map_length; eauto.
         symmetry; eauto.
-        split; eauto.
-        assert (eqns_freeVars e1 [=] eqns_freeVars e1 \ of_list Z) by admit.
-        rewrite H6. symmetry.
+        rewrite sEQ. symmetry.
         eapply update_with_list_agree_minus; eauto. rewrite map_length; eauto.
-        symmetry; eauto.
-        split.
-        rewrite <- H35. clear_all; cset_tac; intuition. 
-        rewrite <- H37. clear_all; cset_tac; intuition.
+        symmetry; eauto. 
         reflexivity.
-        destruct H11. rewrite H11. rewrite eqns_freeVars_union.
-        rewrite H19. rewrite H4. clear_all; cset_tac; intuition.
-        destruct H13. rewrite H13. rewrite eqns_freeVars_union.
-        rewrite H20. rewrite H5. clear_all; cset_tac; intuition.
+        inv H12. rewrite H26; simpl. rewrite H29. rewrite eqns_freeVars_union.
+        rewrite H21. rewrite H4. clear_all; cset_tac; intuition.
+        inv H14. rewrite H29. rewrite H26. simpl. rewrite eqns_freeVars_union.
+        rewrite H22. rewrite H5. clear_all; cset_tac; intuition.
+        subst. eapply agree_on_onvLe; eauto.
       * hnf; split; eauto.
       * unfold entails in *. dcr. hnf; intros.
         simpl. split.
-        rewrite <- H14. cset_tac; intuition. exfalso. eapply H14; eauto.
+        rewrite <- H20. cset_tac; intuition. 
         split.
-        rewrite <- H14. cset_tac; intuition. exfalso. eapply H14; eauto.
-        repeat (split; eauto using agree_on_refl).
-    - destruct H12. rewrite H7; eauto.
-    - destruct H15. rewrite H7; eauto.
+        rewrite H28; reflexivity.
+        repeat (split; eauto; try reflexivity).
+    - inv H13. rewrite H8, H28; eauto.
+    - invc H16. rewrite H8, H28; eauto.
 Qed.
 
 
